WIP Work with Fin
Lean won't unify types for pattern matching because it doesn't want to
reduce ⟦argUserType (Op.and w)⟧. Need to figure out how to force Lean to
do that.

SSA/Examples/InstCombine.lean
@@ -3,161 +3,102 @@ import Aesop
 
 namespace InstCombine
 
-inductive LengthIndexedList (α : Type u) : Nat → Type u where
-   | nil : LengthIndexedList α 0
-   | cons : α → LengthIndexedList α n → LengthIndexedList α (n + 1)
-  deriving Repr, DecidableEq
-
-def LengthIndexedList.fromList {α : Type u} (l : List α) : LengthIndexedList α (List.length l) :=
-  match l with
-  | [] => LengthIndexedList.nil
-  | x :: xs => LengthIndexedList.cons x (LengthIndexedList.fromList xs)
-
-@[simp]
-def LengthIndexedList.foldl {α β : Type u} {n : Nat} (f : β → α → β) (acc : β) : LengthIndexedList α n → β
-  | nil => acc
-  | cons x xs => LengthIndexedList.foldl f (f acc x) xs
-
-@[simp]
-def LengthIndexedList.zipWith {α β γ : Type u} {n : Nat} (f : α → β → γ) :
-    LengthIndexedList α n → LengthIndexedList β n → LengthIndexedList γ n
-  | nil, nil => nil
-  | cons x xs, cons y ys => cons (f x y) (zipWith f xs ys)
-
-abbrev Width := Nat
---
-structure BitVector (width : Width) where
-  (bits : LengthIndexedList Bool width)
-  deriving Repr, DecidableEq
-
-def nextSignificantBit (val : Nat) (b : Bool) := 2 * val + if (b = true) then 1 else 0
-
--- We could instead just define this directly as Fin (2^width)
-def RawBitVectorVal {w : Width} (x : LengthIndexedList Bool w) : Nat :=
-  x.foldl nextSignificantBit 0
-
--- #eval RawBitVectorVal (LengthIndexedList.fromList [false,true]) -- 1
--- #eval RawBitVectorVal (LengthIndexedList.fromList [true,false,false,false]) -- 8
--- #eval RawBitVectorVal $ LengthIndexedList.fromList [true,true,false,false,false] -- 24
--- #eval RawBitVectorVal $ LengthIndexedList.fromList [true,false,false,false, true] -- 17
-#eval RawBitVectorVal $ (LengthIndexedList.fromList [true,false,false,false]).cons true -- 24
-
-theorem nextSignificantBitTrue {val : Nat} : nextSignificantBit val true = 2 * val + 1 := by
-  simp [nextSignificantBit]
-
-theorem nextSignificantBitFalse {val : Nat} : nextSignificantBit val false = 2 * val := by
-  simp [nextSignificantBit]
-
-theorem RawBitVectorFalse {w : Width} {x : LengthIndexedList Bool w} :
-  (LengthIndexedList.cons false x).foldl nextSignificantBit 0 = x.foldl nextSignificantBit 0 := by simp[LengthIndexedList.foldl, nextSignificantBitFalse]
-
-def testExample := fun n => [true,false,true].foldl nextSignificantBit n
-#eval [0,1,2,3,4,5].map testExample
-theorem foldNextSignificantBit {w : Nat} {x : LengthIndexedList Bool w} {v : Nat} :
-  x.foldl nextSignificantBit n = 2^w + x.foldl nextSignificantBit 0 := by
-    induction x with
-      | nil => simp[LengthIndexedList.foldl, nextSignificantBit]
-      | cons b bs ih => simp
-
-
-
-theorem RawBitVectorValNil : RawBitVectorVal (LengthIndexedList.nil) = 0 := by
-  simp [RawBitVectorVal]
-
--- Appends to the most significant bit
-theorem RawBitVectorValConsTrue {w : Width} (x : LengthIndexedList Bool w) (b : Bool) :
-    RawBitVectorVal (x.cons true) =  2 * RawBitVectorVal x + 1 := by
-      simp [RawBitVectorVal, LengthIndexedList.foldl]
-      rw [LengthIndexedList.foldl]
-
-
-
-theorem RawBitVectorValGrowth {w : Width} (x : LengthIndexedList Bool (w - 1)) : ∀ b : Bool, RawBitVectorVal (x.cons b) ≤ 2 * RawBitVectorVal x := by
-  intro b; cases b with
-   | false => simp [RawBitVectorVal]; rw [Nat.two_mul]
-              apply Nat.le_add_left
-   | true => simp [RawBitVectorVal]; unfold LengthIndexedList.foldl <;> cases w
-
-
-theorem BitVector.valRawLT {w : Width} (x : LengthIndexedList Bool w) : RawBitVectorVal x < 2^w := by
-  simp [RawBitVectorVal]
-  induction x with
-  | nil => simp
-  | cons b bs ih => cases b with
-    | false => rw [Nat.pow_succ,Nat.mul_two]
-               apply Nat.lt_add_right
-               simp [LengthIndexedList.foldl] at *
-               exact ih
-    | true => simp  [LengthIndexedList.foldl] at *
-
-
-def BitVector.val {w : Width} (x : BitVector w) : Fin (2^w) :=
-
-
+abbrev Width := { x : Nat // 0 < x } -- difference with { x : Nat  | 0 < x }?
+abbrev BitVector (w : Width) := Fin (2^w)
 inductive BaseType
-  | bitvec (w : Width) : BaseType
+| bitvec (w : Width) : BaseType
 
 instance : Goedel BaseType where
-  toType := fun
-    | .bitvec w => BitVector w
+toType := fun
+  | .bitvec w => BitVector w
 
 abbrev UserType := SSA.UserType BaseType
 
 -- See: https://releases.llvm.org/14.0.0/docs/LangRef.html#bitwise-binary-operations
 inductive Op
-  | and (w : Width) : Op
-  | or (w : Width) : Op
-  | xor (w : Width) : Op
-  | shr (w : Width) : Op
-  | lshr (w : Width) : Op
-  | ashr (w : Width) : Op
-  deriving Repr, DecidableEq
+| and (w : Width) : Op
+| or (w : Width) : Op
+| xor (w : Width) : Op
+| shl (w : Width) : Op
+| lshr (w : Width) : Op
+| ashr (w : Width) : Op
+deriving Repr, DecidableEq
 
 -- Can we get rid of the code repetition here? (not that copilot has any trouble completing this)
+@[reducible]
 def argUserType : Op → UserType
-  | Op.and w => .pair (.base (BaseType.bitvec w)) (.base (BaseType.bitvec w))
-  | Op.or w => .pair (.base (BaseType.bitvec w)) (.base (BaseType.bitvec w))
-  | Op.xor w => .pair (.base (BaseType.bitvec w)) (.base (BaseType.bitvec w))
-  | Op.shr w => .pair (.base (BaseType.bitvec w)) (.base (BaseType.bitvec w))
-  | Op.lshr w => .pair (.base (BaseType.bitvec w)) (.base (BaseType.bitvec w))
-  | Op.ashr w => .pair (.base (BaseType.bitvec w)) (.base (BaseType.bitvec w))
+| Op.and w => .pair (.base (BaseType.bitvec w)) (.base (BaseType.bitvec w))
+| Op.or w => .pair (.base (BaseType.bitvec w)) (.base (BaseType.bitvec w))
+| Op.xor w => .pair (.base (BaseType.bitvec w)) (.base (BaseType.bitvec w))
+| Op.shl w => .pair (.base (BaseType.bitvec w)) (.base (BaseType.bitvec w))
+| Op.lshr w => .pair (.base (BaseType.bitvec w)) (.base (BaseType.bitvec w))
+| Op.ashr w => .pair (.base (BaseType.bitvec w)) (.base (BaseType.bitvec w))
 
 def outUserType : Op → UserType
-  | Op.and w => .base (BaseType.bitvec w)
-  | Op.or w => .base (BaseType.bitvec w)
-  | Op.xor w => .base (BaseType.bitvec w)
-  | Op.shr w => .base (BaseType.bitvec w)
-  | Op.lshr w => .base (BaseType.bitvec w)
-  | Op.ashr w => .base (BaseType.bitvec w)
+| Op.and w => .base (BaseType.bitvec w)
+| Op.or w => .base (BaseType.bitvec w)
+| Op.xor w => .base (BaseType.bitvec w)
+| Op.shl w => .base (BaseType.bitvec w)
+| Op.lshr w => .base (BaseType.bitvec w)
+| Op.ashr w => .base (BaseType.bitvec w)
 
 def rgnDom : Op → UserType := sorry
 def rgnCod : Op → UserType := sorry
 
-def BitVector.bitWiseOp : ∀ {w : Width}, (Bool → Bool → Bool) → BitVector w → BitVector w → BitVector w
-  | _, f, {val := x}, {val := y} => {val := LengthIndexedList.zipWith (fun a b => f a b) x y}
+def BitVector.and : ∀ {w : Width}, BitVector w → BitVector w → BitVector w := (· &&& ·)
+def BitVector.or : ∀ {w : Width}, BitVector w → BitVector w → BitVector w := (· ||| ·)
+def BitVector.xor : ∀ {w : Width}, BitVector w → BitVector w → BitVector w := (· ^^^ ·)
 
-def BitVector.and : ∀ {w : Width}, BitVector w → BitVector w → BitVector w := BitVector.bitWiseOp (· && ·)
-def BitVector.or : ∀ {w : Width}, BitVector w → BitVector w → BitVector w := BitVector.bitWiseOp (· || ·)
-def BitVector.xor : ∀ {w : Width}, BitVector w → BitVector w → BitVector w := BitVector.bitWiseOp (fun a b => (a || b) && (¬ a || ¬ b))
+theorem Nat.zero_lt_pow {m n : Nat} : (0 < n) → 0 < n^m := by
+  induction m with
+  | zero => simp
+  | succ m ih =>
+    intro h
+    rw [Nat.pow_succ]
+    exact Nat.mul_pos (ih h) h
 
--- op1 * 2op2 mod 2n, where n is the width of the result
+theorem Width.zero_lt_pow_2 {w : Width} : 0 < 2^w.val := by
+  have h : 0 < 2 := Nat.zero_lt_succ 1
+  exact @Nat.zero_lt_pow w.val 2 h
+
+def Width.nat_pow (n : Nat) (w : Width) : Nat :=
+ n ^ w
+
+theorem Nat.gt_of_lt {a b : Nat} : a < b → b > a := by simp
+
+def _root_.Nat.asBitVector (n : Nat) {w : Width} : BitVector w :=
+  { val := n % (2^w), isLt := (Nat.mod_lt n w.zero_lt_pow_2) }
+
+def BitVector.shl {w : Width} (op₁ op₂ : BitVector w) : BitVector w :=
+ op₁.val * (2^op₂.val) |>.asBitVector
+
+def BitVector.lshr {w : Width} (op₁ op₂ : BitVector w) : BitVector w := op₁ >>> op₂
+def BitVector.ashr {w : Width} (op₁ op₂ : BitVector w) : BitVector w := op₁ >>> op₂ -- not capturing the difference here obviously
+def BitVector.shl' {w : Width} (op₁ op₂ : BitVector w) : BitVector w := op₁ <<< op₂
+
+
 def eval : ∀ (o : Op), Goedel.toType (argUserType o) → (Goedel.toType (rgnDom o) →
-    Goedel.toType (rgnCod o)) → Goedel.toType (outUserType o) :=
-    fun o arg _ => match o, arg with
-      | Op.and w, .pair x y => fun (x y : BitVector w) => .base {val := (LengthIndexedList.zipWith (fun a b => a && b) x.val y.val)}
+  Goedel.toType (rgnCod o)) → Goedel.toType (outUserType o) :=
+  fun o arg _ => match o, arg with
+    | Op.and w, SSA.UserType.pair x y => fun (x y : BitVector w) => UserType.base $ BitVector.and x y
+    | Op.or w, SSA.UserType.pair x y => fun (x y : BitVector w) => UserType.base $ BitVector.or x y
+    | Op.xor w, SSA.UserType.pair x y => fun (x y : BitVector w) => UserType.base $ BitVector.xor x y
+    | Op.lshr w, SSA.UserType.pair x y => fun (x y : BitVector w) => UserType.base $ BitVector.lshr x y
+    | Op.ashr w, SSA.UserType.pair x y => fun (x y : BitVector w) => UserType.base $ BitVector.ashr x y
+    | Op.shl w, SSA.UserType.pair x y => fun (x y : BitVector w) => UserType.base $ BitVector.shl x y
 
 instance : SSA.TypedUserSemantics Op BaseType where
-  argUserType := argUserType
-  rgnDom := rgnDom
-  rgnCod := rgnCod
-  outUserType := outUserType
-  eval := eval
+argUserType := argUserType
+rgnDom := rgnDom
+rgnCod := rgnCod
+outUserType := outUserType
+eval := eval
 
-end InstCombine
 /-
 Optimization: InstCombineShift: 239
-  %Op0 = shl %X, C
-  %r = lshr %Op0, C
+%Op0 = shl %X, C
+%r = lshr %Op0, C
 =>
-  %r = and %X, (-1 u>> C)
+%r = and %X, (-1 u>> C)
 -/
+end InstCombine
